Nemonuri/PropositionalLogics/Basic.lean
@@ -1,0 +1,1186 @@
+module
+
+public import Mathlib.Data.Fintype.Basic
+public import Mathlib.Data.Fintype.Pi
+public import Mathlib.Data.Finite.Prod
+public import Mathlib.Data.Setoid.Basic
+
+/-!
+
+## References
+
+* [Christel Baier, Joost-Pieter Katoen, *Principles of Model Checking*][PoMC], A.3 Propositional Logic, p.915
+
+-/
+
+@[expose] public section
+
+namespace Nemonuri.PropositionalLogics
+
+
+inductive Formula (AP: Type _) [Fintype AP] where
+  | true
+  | atom (x: AP)
+  | neg (x: Formula AP)
+  | and (x: Formula AP) (y: Formula AP)
+
+/-
+@[mk_iff]
+inductive IsFormula (AP: Type _) [Fintype AP] : (FormulaRaw AP) → Prop where
+  | true : IsFormula AP (.true)
+  | atom (x: AP) : IsFormula AP (.atom x)
+  | neg (x: FormulaRaw AP) (hx: IsFormula AP x) : IsFormula AP (.neg x)
+  | and (x: FormulaRaw AP) (y: FormulaRaw AP)
+        (hx: IsFormula AP x) (hy: IsFormula AP y) : IsFormula AP (.and x y)
+
+@[ext]
+structure Formula (AP: Type _) [Fintype AP] where
+  raw: FormulaRaw AP
+  valid: IsFormula AP raw
+-/
+
+
+namespace Formula
+
+variable {AP: Type _} [Fintype AP]
+
+instance toNonempty : Nonempty (Formula AP) := .intro .true
+
+theorem ne_atom_of_empty_ap [IsEmpty AP] {p: Formula AP} {ap: AP} : (p ≠ .atom ap) := by
+  intro lm1
+  cases p <;> try simp at lm1
+  exact (inferInstance: IsEmpty AP).false ap
+
+theorem exists_eq_atom_iff_nonempty : (∃(p: Formula AP), ∃(ap: AP), p = .atom ap) ↔ Nonempty AP := by
+  constructor
+  · rintro ⟨p, ap, lm1⟩
+    exact .intro ap
+  · rintro ⟨ap⟩
+    exists .atom ap
+    exists ap
+
+def hasAtom : Formula AP → Bool
+  | .true => .false
+  | .atom _ => .true
+  | .neg p => hasAtom p
+  | .and p1 p2 => (hasAtom p1) || (hasAtom p2)
+
+@[simp]
+theorem and_hasAtom_eq_false_iff_hasAtom_eq_false_and {p1 p2: Formula AP}
+  : ((p1.and p2).hasAtom = .false) ↔ (p1.hasAtom = false) ∧ (p2.hasAtom = false) := by
+  simp [hasAtom]
+
+
+
+def collectAtom [DecidableEq AP] : Formula AP → Finset AP
+  | .true => ∅
+  | .atom ap => {ap}
+  | .neg p => collectAtom p
+  | .and p1 p2 => (collectAtom p1) ∪ (collectAtom p2)
+
+
+theorem hasAtom_eq_true_iff_collectAtom_nonempty [DecidableEq AP] {p: Formula AP}
+  : p.hasAtom = .true ↔ p.collectAtom.Nonempty := by
+  rcases p with _ | ap | p | ⟨p1, p2⟩
+  · dsimp [hasAtom, collectAtom]; simp
+  · dsimp [hasAtom, collectAtom]; simp
+  · dsimp [hasAtom, collectAtom]
+    exact @p.hasAtom_eq_true_iff_collectAtom_nonempty _
+  · dsimp [hasAtom, collectAtom]
+    simp
+    have lm1 := @p1.hasAtom_eq_true_iff_collectAtom_nonempty _
+    have lm2 := @p2.hasAtom_eq_true_iff_collectAtom_nonempty _
+    rw [lm1, lm2]
+
+
+theorem hasAtom_eq_false_of_ap_empty [IsEmpty AP] {p: Formula AP} : p.hasAtom = .false := by
+  by_contra lm1
+  simp at lm1
+  let deqAP : DecidableEq AP := Classical.typeDecidableEq AP
+  have lm2 := p.hasAtom_eq_true_iff_collectAtom_nonempty
+  replace lm2 := lm2.mp lm1 |> Finset.nonempty_def.mp
+  rcases lm2 with ⟨ap, lm2⟩
+  exact (inferInstance : IsEmpty AP).false ap
+
+
+def evalToBool? (p: Formula AP) : Option Bool := do
+  match p with
+  | .true => return .true
+  | .atom _ => .none
+  | .neg p => return !(← p.evalToBool?)
+  | .and p1 p2 => return (← p1.evalToBool?) && (← p2.evalToBool?)
+
+theorem evalToBool?_isSome_of_hasAtom_eq_false (p: Formula AP) (req: p.hasAtom = .false) : p.evalToBool?.isSome = .true := by
+  rcases p with _ | ap | p | ⟨p1, p2⟩
+  · dsimp [evalToBool?]
+  · dsimp [hasAtom] at req
+    simp at req
+  · dsimp [hasAtom] at req
+    dsimp [evalToBool?]
+    cases lm1: p.evalToBool?
+    · simp
+      have lm2 := p.evalToBool?_isSome_of_hasAtom_eq_false req
+      simp [lm1] at lm2
+    · simp
+  · dsimp [hasAtom] at req
+    dsimp [evalToBool?]
+    simp at req
+    rcases req with ⟨req1, req2⟩
+    cases lm1: p1.evalToBool?
+    · have lm2 := p1.evalToBool?_isSome_of_hasAtom_eq_false req1
+      simp [lm1] at lm2
+    · simp
+      cases lm2: p2.evalToBool?
+      · have lm3 := p2.evalToBool?_isSome_of_hasAtom_eq_false req2
+        simp [lm2] at lm3
+      · simp
+
+def evalToBool (p: Formula AP) (req: p.hasAtom = .false) : Bool :=
+  match lm1: p.evalToBool? with
+  | .some val => val
+  | .none => absurd lm1 (by
+      have lm2 := p.evalToBool?_isSome_of_hasAtom_eq_false req
+      simp [lm1] at lm2 )
+
+theorem evalToBool_eq_iff_evalToBool?_eq_some {p: Formula AP} (req: p.hasAtom = .false) {b: Bool}
+  : (p.evalToBool req = b) ↔ (p.evalToBool? = .some b) := by
+  have lm1 := p.evalToBool?_isSome_of_hasAtom_eq_false req
+  dsimp [evalToBool]
+  split <;> (rename_i lm2; simp [lm2] at lm1)
+  rw [lm2]
+  exact Option.some_inj.symm
+
+
+/-
+protected def mk' (AP: Type _) [Fintype AP] (x: FormulaRaw AP) (h: IsFormula AP x) : Formula AP := @Formula.mk AP _ x h
+
+@[match_pattern]
+protected def true (AP: Type _) [Fintype AP] : Formula AP := ⟨.true, .true⟩
+
+@[match_pattern]
+protected def atom (x: AP) : Formula AP := ⟨.atom x, .atom x⟩
+
+@[match_pattern]
+protected def neg (x: Formula AP) : Formula AP := ⟨.neg x.raw, .neg x.raw x.valid⟩
+
+@[match_pattern]
+protected def and (x y: Formula AP) : Formula AP := ⟨.and x.raw y.raw, .and x.raw y.raw x.valid y.valid⟩
+
+@[elab_as_elim]
+protected def recAlt
+  {motive : Formula AP → Sort _}
+  (true : motive <| Formula.true AP)
+  (atom : (x: AP) → motive <| Formula.atom x)
+  (neg : (x: Formula AP) → motive <| Formula.neg x)
+  (and : (x y: Formula AP) → motive <| Formula.and x y)
+  (t: Formula AP)
+  : motive t :=
+  let ⟨raw, valid⟩ := t
+  match raw with
+  | .true => true
+  | .atom x => atom x
+  | .neg x => neg (.mk' AP x (by cases valid; assumption))
+  | .and x y => and (.mk' AP x (by cases valid; assumption)) (.mk' AP y (by cases valid; assumption))
+-/
+
+/-
+inductive Splitted (AP: Finset Atom) : Formula AP → Type _ where
+  | true : Splitted AP (.true AP)
+  | atom (x: AP) : Splitted AP (.atom AP x)
+  | neg (x: Formula AP) : Splitted AP (.neg x)
+  | and (x y: Formula AP) : Splitted AP (.and x y)
+
+def split (x: Formula AP) : Splitted AP x :=
+  Formula.recAlt Splitted.true Splitted.atom Splitted.neg Splitted.and x
+-/
+
+protected def or (x y: Formula AP) : Formula AP := .and (.neg x) (.neg y) |> .neg
+
+protected def imp (x y: Formula AP) : Formula AP := .or (.neg x) y
+
+protected def eqv (x y: Formula AP) : Formula AP := .or (.and (.neg x) (.neg y)) (.and x y)
+
+protected def false : Formula AP := .neg (.true)
+
+def iterAnd (xs: List (Formula AP)) : Formula AP :=
+  match xs with
+  | [] => (.true)
+  | hd::tl => .and hd (iterAnd tl)
+
+def iterOr (xs: List (Formula AP)) : Formula AP :=
+  match xs with
+  | [] => (.false)
+  | hd::tl => .or hd (iterOr tl)
+
+
+section Notation
+
+syntax:42 " ¬ₚ" term:42 : term
+syntax:36 term:37 " ∧ₚ " term:36 : term
+syntax:35 term:36 " ∨ₚ " term:35 : term
+syntax:31 term:32 " →ₚ " term:31 : term
+syntax:30 term:31 " ↔ₚ " term:30 : term
+syntax:41 " ⋀ₚ" term:41 : term
+syntax:41 " ⋁ₚ" term:41 : term
+
+macro_rules
+  | `(¬ₚ$x) => ``(Formula.neg $x)
+  | `($x ∧ₚ $y) => ``(Formula.and $x $y)
+  | `($x ∨ₚ $y) => ``(Formula.or $x $y)
+  | `($x →ₚ $y) => ``(Formula.imp $x $y)
+  | `($x ↔ₚ $y) => ``(Formula.equiv $x $y)
+  | `(⋀ₚ$xs) => ``(iterAnd $xs)
+  | `(⋁ₚ$xs) => ``(iterOr $xs)
+
+end Notation
+
+def atomTuple (as: List AP) : Formula AP := iterAnd (as.map (Formula.atom))
+
+end Formula
+
+
+structure Eval (AP: Type _) [Fintype AP] where
+  eval : AP → Bool
+
+namespace Eval
+
+variable {AP: Type _} [Fintype AP]
+
+instance : FunLike (Eval AP) AP Bool where
+  coe μ := μ.eval
+  coe_injective μ1 μ2 := by cases μ1; cases μ2; simp
+
+theorem app_eq_eval_app (μ: Eval AP) (a: AP) : μ a = μ.eval a := by rfl
+
+end Eval
+
+abbrev Indicator (AP: Type _) [Fintype AP] : Type _ := AP → Bool
+
+@[defeq]
+theorem indicator_def {AP: Type _} [Fintype AP] : Indicator AP = (AP → Bool) := rfl
+
+namespace Indicator
+
+variable {AP: Type _} [Fintype AP]
+
+def mk (f: AP → Bool) : Indicator AP := f
+
+def fn (ind: Indicator AP) : AP → Bool := ind
+
+@[defeq, simp]
+theorem mk_fn_eq {f: AP → Bool} : (mk f).fn = f := rfl
+
+@[defeq, simp]
+theorem mk_eq {f: AP → Bool} {ap: AP} : (mk f) ap = f ap := rfl
+
+
+def evalFormulaToBool (ind: Indicator AP) (p: Formula AP) : Bool :=
+  match p with
+  | .true => .true
+  | .atom ap => ind.fn ap
+  | .neg p => !(ind.evalFormulaToBool p)
+  | .and p1 p2 => (ind.evalFormulaToBool p1) && (ind.evalFormulaToBool p2)
+
+
+open Formula in
+theorem evalFormulaToBool_eq_evalToBool_of_ap_empty [IsEmpty AP] {ind: Indicator AP} {p: Formula AP}
+  : ind.evalFormulaToBool p = p.evalToBool (p.hasAtom_eq_false_of_ap_empty) := by
+  have lm1 := p.hasAtom_eq_false_of_ap_empty
+  have lm2 := p.evalToBool?_isSome_of_hasAtom_eq_false lm1 |> Option.isSome_iff_exists.mp
+  rcases lm2 with ⟨val, lm2⟩
+  rcases p with _ | ap | p | ⟨p1, p2⟩
+  · dsimp [evalFormulaToBool, evalToBool, evalToBool?]
+  · revert ap; simp only [IsEmpty.forall_iff]
+  · dsimp [evalFormulaToBool]
+    have lm3 := @evalFormulaToBool_eq_evalToBool_of_ap_empty _ ind p |>.symm
+    rewrite [p.evalToBool_eq_iff_evalToBool?_eq_some] at lm3
+    have lm4 := lm2
+    dsimp [evalToBool?] at lm4
+    simp [lm3] at lm4
+    symm
+    rw [p.neg.evalToBool_eq_iff_evalToBool?_eq_some, lm2, lm4]
+    simp
+  · obtain ⟨lm1_1, lm1_2⟩ := and_hasAtom_eq_false_iff_hasAtom_eq_false_and.mp lm1
+    clear lm1
+    have lm3_1 := @evalFormulaToBool_eq_evalToBool_of_ap_empty _ ind p1 |>.symm
+    have lm3_2 := @evalFormulaToBool_eq_evalToBool_of_ap_empty _ ind p2 |>.symm
+    rewrite [evalToBool_eq_iff_evalToBool?_eq_some] at lm3_1 lm3_2
+    have lm4 := lm2
+    dsimp [evalToBool?] at lm4
+    rewrite [lm3_1, lm3_2] at lm4
+    simp at lm4
+    dsimp [evalFormulaToBool]
+    symm
+    rw [lm4, evalToBool_eq_iff_evalToBool?_eq_some]
+    exact lm2
+
+
+structure AreEvalToTrue (ind: Indicator AP) (p: Formula AP) : Prop where
+  intro :: eq_true : evalFormulaToBool ind p = .true
+
+namespace AreEvalToTrue
+
+variable {ind: Indicator AP} {p: Formula AP}
+
+theorem eq_true_iff : (evalFormulaToBool ind p = .true) ↔ (AreEvalToTrue ind p) := by
+  constructor
+  · intro lm1
+    exact .intro lm1
+  · rintro ⟨lm1⟩
+    exact lm1
+
+end AreEvalToTrue
+
+
+
+/-
+    have lm3 := @evalFormulaToBool_eq_evalToBool_of_ap_empty _ ind p |>.symm
+    rewrite [p.evalToBool_eq_iff_evalToBool?_eq_some] at lm3
+    symm
+    rw [p.neg.evalToBool_eq_iff_evalToBool?_eq_some, lm2]
+-/
+/-
+    simp
+    have lm3 := @evalFormulaToBool_eq_evalToBool_of_ap_empty _ ind p
+    refine Eq.trans lm3 ?_
+    obtain ⟨_, lm4⟩ := p.evalToBool?_isSome_of_hasAtom_eq_false lm1 |> Option.isSome_iff_exists.mp
+    dsimp [evalToBool] at lm3
+    split at lm3 <;> (rename_i lm5; simp [lm4] at lm5)
+-/
+
+    --dsimp [evalToBool]
+
+
+
+
+scoped instance [DecidableEq AP] : Fintype (AP → Bool) := Pi.instFintype
+
+instance toFintype [DecidableEq AP] : Fintype (Indicator AP) := inferInstanceAs (Fintype (AP → Bool))
+
+instance toFinite : Finite (Indicator AP) := letI := Classical.typeDecidableEq AP; Finite.of_fintype (Indicator AP)
+
+instance toNonempty : Nonempty (Indicator AP) := inferInstanceAs (Nonempty (AP → Bool))
+
+instance uniqueOfIsEmpty [IsEmpty AP] : Unique (Indicator AP) := Pi.uniqueOfIsEmpty (fun _ => Bool)
+
+
+def forallRightEquiv (α: Sort _) : (α → Indicator AP) ≃ (α → AP → Bool) where
+  toFun x := x
+  invFun x := x
+
+@[simps]
+def forallRightEquivOfEquiv {Ind: Sort _} (eqv: Indicator AP ≃ Ind) (α: Sort _) : (α → Indicator AP) ≃ (α → Ind) where
+  toFun f a := eqv (f a)
+  invFun f a := eqv.symm (f a)
+  left_inv := by intro _; simp
+  right_inv := by intro _; simp
+
+def equivToEval : Indicator AP ≃ Eval AP where
+  toFun := Eval.mk
+  invFun := Eval.eval
+
+
+def toFinset (ind: Indicator AP) : Finset AP := { ap: AP | ind.fn ap = .true }
+
+section OfFinset
+
+variable [DecidableEq AP]
+
+def ofFinset (fs: Finset AP) : Indicator AP := .mk (fun ap => decide (ap ∈ fs))
+
+theorem ofFinset_toFinset_leftInverse : Function.LeftInverse (@ofFinset AP _ _) toFinset := by
+  dsimp [Function.LeftInverse, ofFinset, toFinset]
+  dsimp [Indicator, fn, mk]
+  simp
+
+theorem ofFinset_toFinset_rightInverse : Function.RightInverse (@ofFinset AP _ _) toFinset := by
+  dsimp [Function.RightInverse, Function.LeftInverse, ofFinset, toFinset]
+  simp
+
+@[simps]
+def equivToFinset : Indicator AP ≃ Finset AP where
+  toFun := toFinset
+  invFun := ofFinset
+  left_inv := ofFinset_toFinset_leftInverse
+  right_inv := ofFinset_toFinset_rightInverse
+
+
+end OfFinset
+
+end Indicator
+
+
+namespace Eval
+
+variable {AP: Type _} [Fintype AP]
+
+instance toFintype [DecidableEq AP] : Fintype (Eval AP) := Fintype.ofEquiv (Indicator AP) Indicator.equivToEval
+
+instance to_finite : Finite (Eval AP) := letI := Classical.typeDecidableEq AP; Finite.of_fintype (Eval AP)
+
+instance to_nonempty : Nonempty (Eval AP) := Equiv.nonempty Indicator.equivToEval.symm
+
+instance uniqueOfAPEmpty [IsEmpty AP] : Unique (Eval AP) := Equiv.unique Indicator.equivToEval.symm
+
+
+theorem all_eq_of_ap_empty [IsEmpty AP] {ev1 ev2: Eval AP} : ev1 = ev2 := (inferInstance: Unique (Eval AP)).instSubsingleton.allEq ev1 ev2
+
+
+theorem subset_finite {ss: Set (Eval AP)} : ss.Finite := by
+  have lm1 : Finite (Eval AP) := to_finite
+  rw [← Set.finite_coe_iff]
+  exact Subtype.finite
+
+
+
+end Eval
+
+
+
+
+class EvalLike (E: Type _) (AP: outParam <| Type _) [Fintype AP] where
+  protected coe (e: E) : Eval AP
+  coe_injective : Function.Injective coe
+  --coe_surjective : Function.Surjective coe
+
+namespace EvalLike
+
+attribute [coe] EvalLike.coe
+
+variable {E: Type _} {AP: Type _} [Fintype AP] [EvalLike E AP]
+
+instance : CoeOut E (Eval AP) where coe := EvalLike.coe
+
+abbrev toIndicator (e: E) : Indicator AP := .mk ((e: Eval AP) : AP → Bool)
+
+def toIndicator_def {e: E} : (toIndicator e) = .mk ((e: Eval AP).eval) := rfl
+
+
+abbrev AreEvalToTrueAt (E AP: Type _) [Fintype AP] [EvalLike E AP] : E → Formula AP → Prop := Indicator.AreEvalToTrue ∘ toIndicator
+
+@[defeq]
+theorem areEvalToTrueAt_eq_areEvalToTrue {e: E} {p: Formula AP} : AreEvalToTrueAt E AP e p = (toIndicator e).AreEvalToTrue p := rfl
+
+
+instance finite_of_carrier : Finite E := Finite.of_injective EvalLike.coe EvalLike.coe_injective
+
+instance coe_finite : Finite (E → (Eval AP)) := Pi.finite
+
+instance to_finite : Finite (EvalLike E AP) := by
+  let invMk (e: EvalLike E AP) : E → (Eval AP) := e.coe
+  refine Finite.of_injective invMk ?_
+  subst invMk
+  rintro ⟨el1_1, el1_2⟩ ⟨el2_1, el2_2⟩
+  simp
+  intro lm1
+  congr
+
+
+instance coeUniqueOfAPEmpty [IsEmpty AP] : Unique (E → (Eval AP)) := Pi.unique
+
+
+theorem coe_eq_of_ap_empty [IsEmpty AP] {E2: Type _} [EvalLike E2 AP] {e: E} (e2: E2) : (e: Eval AP) = (e2: Eval AP) := Eval.all_eq_of_ap_empty
+
+
+
+def RangeAt (E AP: Type _) [Fintype AP] [EvalLike E AP] : Set (Eval AP) := Set.range (@EvalLike.coe E AP _ _)
+
+theorem rangeAt_finite : (RangeAt E AP).Finite := Eval.subset_finite
+
+theorem rangeAt_eq_empty_of_carrier_empty [IsEmpty E] : (RangeAt E AP) = ∅ := by
+  dsimp [RangeAt]
+  rw [Set.range_eq_empty_iff]
+  exact inferInstance
+
+theorem rangeAt_eq_empty_iff_carrier_empty : ((RangeAt E AP) = ∅) ↔ (IsEmpty E) := by
+  constructor
+  · intro lm1
+    dsimp [RangeAt] at lm1
+    exact Set.range_eq_empty_iff.mp lm1
+  · exact @rangeAt_eq_empty_of_carrier_empty E AP _ _
+
+
+theorem rangeAt_eq_singleton_of_carrier_nonempty_and_ap_empty [Nonempty E] [IsEmpty AP]
+  : (RangeAt E AP) = {(default: Eval AP)} := by
+  dsimp [RangeAt, Inhabited.default, Indicator.equivToEval]
+  simp only [Set.range_eq_singleton_iff]
+  intro c
+  exact Eval.all_eq_of_ap_empty
+
+
+theorem rangeAt_empty_or_singleton_of_ap_empty [IsEmpty AP]
+  : ((RangeAt E AP) = ∅) ∨ ((RangeAt E AP) = {(default: Eval AP)}) := by
+  have lm1 := isEmpty_or_nonempty E
+  rcases lm1 with lm1 | lm1
+  · have lm2 := rangeAt_eq_empty_iff_carrier_empty.mpr lm1
+    exact Or.inl lm2
+  · have lm2 := @rangeAt_eq_singleton_of_carrier_nonempty_and_ap_empty E AP _ _ _ _
+    exact Or.inr lm2
+
+
+
+
+
+variable [DecidableEq AP]
+
+/-
+scoped instance (A: Finset AP) (a: AP) : Decidable (a ∈ A) := A.decidableMem a
+
+def ofSubset (A: Finset AP) : Eval AP := ⟨fun a => decide (a ∈ A)⟩
+
+theorem ofSubset_injective : Function.Injective (@ofSubset AP _ _) := by
+  intro a1 a2
+  unfold ofSubset
+  simp
+  intro lm1
+  rewrite [funext_iff] at lm1
+  ext a
+  specialize lm1 a
+  simpa only [decide_eq_decide] using lm1
+
+theorem ofSubset_surjective : Function.Surjective (@ofSubset AP _ _) := by
+  rintro ⟨a⟩
+  dsimp [ofSubset]
+  let a1 : Finset AP := Finset.univ.filter (a · = .true)
+  exists a1
+  subst a1
+  refine congrArg _ ?_
+  refine funext ?_; intro ap
+  simp
+-/
+
+open Indicator in
+instance : EvalLike (Finset AP) AP where
+  coe := Eval.mk ∘ Indicator.fn ∘ equivToFinset.symm
+  coe_injective := by intro _ _; simp [Indicator.fn]
+
+
+instance : EvalLike (AP → Bool) AP where
+  coe := Eval.mk
+  coe_injective := by intro _ _; simp
+  --coe_surjective := by rintro ⟨a⟩; exists a
+
+instance (priority := 10) : EvalLike (Eval AP) AP where
+  coe := id
+  coe_injective := Function.injective_id
+
+omit [DecidableEq AP] in
+@[reducible]
+def ofKerLift (toInd: E → AP → Bool) : EvalLike (Quotient (Setoid.ker toInd)) AP where
+  coe qe := Setoid.kerLift toInd qe |> Eval.mk
+  coe_injective := by
+    have lm1 := @Setoid.kerLift_injective _ _ toInd
+    intro _ _
+    simp
+    exact lm1.eq_iff.mp
+
+end EvalLike
+
+
+
+/-
+structure SatRelRaw (AP: Type _) [Fintype AP] where
+  ofRel :: rel : Eval AP → Formula AP → Prop
+
+instance : FunLike (SatRelRaw AP) (Eval AP) (Formula AP → Prop) where
+  coe x := x.rel
+  coe_injective x1 x2 := by cases x1; cases x2; simp
+
+@[mk_iff]
+structure IsSatRel (AP: Type _) [Fintype AP] (raw: SatRelRaw AP) : Prop where
+  true : ∀μ, raw μ (.true AP)
+  atom (a: AP) : ∀μ, raw μ (.atom a) ↔ (μ a = .true)
+  neg (x: Formula AP) : ∀μ, raw μ (¬ₚx) ↔ (¬raw μ x)
+  and (x y: Formula AP) : ∀μ, raw μ (x ∧ₚ y) ↔ (raw μ x ∧ raw μ y)
+
+structure SatRel (AP: Type _) [Fintype AP] where
+  raw: SatRelRaw AP
+  valid: IsSatRel AP raw
+
+instance : FunLike (SatRel AP) (Eval AP) (Formula AP → Prop) where
+  coe x := x.raw
+  coe_injective x1 x2 := by cases x1; cases x2; simp
+-/
+
+@[mk_iff]
+structure IsSatRelAt (AP: Type _) [Fintype AP] (C: Type _) (eval: C → AP → Bool) (rel: C → Formula AP → Prop) : Prop where
+  true (μ: C) : rel μ (.true)
+  atom (μ: C) (a: AP) : rel μ (.atom a) ↔ (eval μ a = .true)
+  neg (μ: C) (x: Formula AP) : rel μ (¬ₚx) ↔ (¬rel μ x)
+  and (μ: C) (x y: Formula AP) : rel μ (x ∧ₚ y) ↔ (rel μ x ∧ rel μ y)
+
+namespace IsSatRelAt
+
+variable {AP: Type _} [Fintype AP]
+         {C: Type _} {eval: C → AP → Bool} {rel: C → Formula AP → Prop}
+         {C2: Type _} {eval2: C2 → AP → Bool} {rel2: C2 → Formula AP → Prop}
+
+theorem of_carrier_empty [IsEmpty C] : IsSatRelAt AP C eval rel := by constructor <;> simp
+
+open EvalLike Indicator in
+theorem of_eq_areEvalToTrue [EvalLike C AP] (req: rel = AreEvalToTrueAt C AP) : IsSatRelAt AP C toIndicator rel := by
+  simp only [funext_iff, areEvalToTrueAt_eq_areEvalToTrue, ← AreEvalToTrue.eq_true_iff] at req
+  constructor
+  · intro c
+    specialize req c Formula.true
+    dsimp [evalFormulaToBool] at req
+    simpa using req
+  · intro c ap
+    specialize req c (Formula.atom ap)
+    dsimp [evalFormulaToBool, Indicator.fn] at req
+    exact req |> propext_iff.mp
+  · intro c p
+    have lm1 := req c p
+    have lm2 := req c p.neg
+    dsimp [evalFormulaToBool, Indicator.fn] at lm2
+    rw [lm2, lm1]
+    simp
+  · intro c p1 p2
+    have lm1 := req c p1
+    have lm2 := req c p2
+    have lm3 := req c (p1.and p2)
+    dsimp [evalFormulaToBool, Indicator.fn] at lm3
+    simp at lm3
+    rw [lm3, lm2, lm1]
+
+open EvalLike Indicator in
+theorem to_eq_areEvalToTrue_at [EvalLike C AP] (h: IsSatRelAt AP C toIndicator rel) (c: C) (p: Formula AP) : rel c p ↔ AreEvalToTrueAt C AP c p := by
+  simp only [areEvalToTrueAt_eq_areEvalToTrue, ← AreEvalToTrue.eq_true_iff]
+  obtain ⟨lm1_true, lm1_atom, lm1_neg, lm1_and⟩ := id h
+  rcases p with _ | ap | p | ⟨p1, p2⟩
+  · simp [evalFormulaToBool]
+    exact lm1_true c
+  · dsimp [evalFormulaToBool, Indicator.fn]
+    exact lm1_atom c ap
+  · have lm2 := h.to_eq_areEvalToTrue_at c p
+    simp only [areEvalToTrueAt_eq_areEvalToTrue, ← AreEvalToTrue.eq_true_iff] at lm2
+    have lm3 := lm1_neg c p
+    dsimp [evalFormulaToBool, Indicator.fn]
+    rw [lm3, lm2]
+    simp
+  · have lm2_1 := h.to_eq_areEvalToTrue_at c p1
+    have lm2_2 := h.to_eq_areEvalToTrue_at c p2
+    simp only [areEvalToTrueAt_eq_areEvalToTrue, ← AreEvalToTrue.eq_true_iff] at lm2_1 lm2_2
+    simp [evalFormulaToBool]
+    rw [← lm2_1, ← lm2_2]
+    have lm3 := lm1_and c p1 p2
+    exact lm3
+
+open EvalLike in
+theorem to_eq_areEvalToTrue [EvalLike C AP] (h: IsSatRelAt AP C toIndicator rel) : rel = AreEvalToTrueAt C AP := by
+  simp only [funext_iff, propext_iff]
+  exact h.to_eq_areEvalToTrue_at
+
+open EvalLike in
+theorem eq_areEvalToTrue_iff [EvalLike C AP] : (IsSatRelAt AP C toIndicator rel) ↔ (rel = AreEvalToTrueAt C AP) :=
+  ⟨to_eq_areEvalToTrue, of_eq_areEvalToTrue⟩
+
+
+
+/-
+open EvalLike Indicator in
+theorem iff_iff_toEvalFormulaToBool_eq_true [EvalLike C AP]
+  : (∀c p, rel c p ↔ toEvalFormulaToBool c p = .true) ↔ IsSatRelAt AP C toIndicator rel := by
+  constructor
+  · exact of_iff_toEvalFormulaToBool_eq_true
+  · intro lm1 c p
+    have lm1_1 := lm1
+    dsimp [toEvalFormulaToBool]
+    rcases lm1 with ⟨lm1_true, lm1_atom, lm1_neg, lm1_and⟩
+    rcases p with _ | ap | p | ⟨p1, p2⟩
+    · simp [evalFormulaToBool]
+      exact lm1_true c
+    · dsimp [evalFormulaToBool, Indicator.fn]
+      exact lm1_atom c ap
+    · dsimp [evalFormulaToBool, Indicator.fn]
+      have lm2 := lm1_neg c p
+-/
+
+
+
+  --dsimp [EvalToFormulaSetAt] at req
+  --simp [Set.ext_iff] at req
+
+/-
+theorem of_ap_empty_at [IsEmpty AP] (req1: ∀(c: C), rel c .true) : IsSatRelAt AP C eval rel := by
+  constructor
+  · exact req1
+  · intro _; simp only [IsEmpty.forall_iff]
+  · intro c p
+    rcases p with _ | ap | p | ⟨p1, p2⟩
+    · simp [req1]; revert c
+-/
+
+def SetOfValidFormula (_: IsSatRelAt AP C eval rel) : Set (Formula AP) := { p: Formula AP | ∃(c: C), rel c p }
+
+
+/-
+open EvalLike in
+theorem rangeAt_eq_iff_valid_formula_eq_of_ap_empty [IsEmpty AP]
+  [EvalLike C AP] [EvalLike C2 AP] (req1: IsSatRelAt AP C toIndicator rel) (req2: IsSatRelAt AP C2 toIndicator rel2)
+  : (RangeAt C AP = RangeAt C2 AP) ↔ (req1.SetOfValidFormula = req2.SetOfValidFormula) := by
+  have lm1 := fun ev1 => @Eval.all_eq_of_ap_empty AP _ _ ev1 (default: Eval AP)
+  dsimp [SetOfValidFormula]
+  unfold toIndicator at req1 req2
+  simp [lm1, DFunLike.coe] at req1 req2
+  rcases req1 with ⟨req1_true, req1_atom, req1_neg, req1_and⟩
+  rcases req2 with ⟨req2_true, req2_atom, req2_neg, req2_and⟩
+  simp at req1_atom req2_atom
+  clear req1_atom req2_atom
+  dsimp [RangeAt]
+  simp [Set.ext_iff]
+  constructor
+  · intro lm2 p
+    specialize lm2 (default: Eval AP)
+    simp [lm1] at lm2
+-/
+/-
+    constructor
+    · rintro ⟨c, lm3⟩
+      specialize lm2 (c: Eval AP)
+      simp at lm2
+      rcases lm2 with ⟨c2, lm2⟩
+-/
+
+
+/-
+  constructor
+  · intro lm2
+    dsimp [RangeAt] at lm2
+    dsimp [SetOfValidFormula]
+    simp [Set.ext_iff] at lm2 ⊢
+    intro p
+    constructor
+    · rintro ⟨c, lm3⟩
+      specialize lm2 (c: Eval AP)
+      simp at lm2
+      rcases lm2 with ⟨c2, lm2⟩
+-/
+
+/-
+open EvalLike in
+theorem rangeAt_eq_iff_valid_formula_eq
+  [EvalLike C AP] [EvalLike C2 AP] (req1: IsSatRelAt AP C toIndicator rel) (req2: IsSatRelAt AP C2 toIndicator rel2)
+  : (RangeAt C AP = RangeAt C2 AP) ↔ (req1.SetOfValidFormula = req2.SetOfValidFormula) := by
+  --unfold toIndicator at req1 req2
+  constructor
+  · intro lm1
+    dsimp [RangeAt] at lm1
+    dsimp [SetOfValidFormula]
+    simp [Set.ext_iff] at lm1 ⊢
+    intro p
+    constructor
+    · rintro ⟨c, lm2⟩
+      specialize lm1 (c: Eval AP)
+      simp at lm1
+      rcases lm1 with ⟨c2, lm3⟩
+      exists c2
+      unfold toIndicator at req1 req2
+      rcases req1 with ⟨req1_true, req1_atom, req1_neg, req1_and⟩
+      replace req1_true := req1_true c
+      replace req1_atom := fun a => req1_atom a c
+      replace req1_neg := fun a => req1_neg a c
+      replace req1_and := fun a1 a2 => req1_and a1 a2 c
+      rcases req2 with ⟨req2_true, req2_atom, req2_neg, req2_and⟩
+      replace req2_true := req2_true c2
+      replace req2_atom := fun a => req2_atom a c2
+      replace req2_neg := fun a => req2_neg a c2
+      replace req2_and := fun a1 a2 => req2_and a1 a2 c2
+      have lm4 := isEmpty_or_nonempty AP
+      rcases lm4 with lm4 | lm4
+      · simp only [IsEmpty.forall_iff] at req1_atom req2_atom
+        clear req1_atom req2_atom
+-/
+      --rcases req2 with ⟨req2_true, req2_atom, req2_neg, req2_and⟩
+/-
+    rcases req1 with ⟨req1_true, req1_atom, req1_neg, req1_and⟩
+    rcases req2 with ⟨req2_true, req2_atom, req2_neg, req2_and⟩
+    constructor
+    · rintro ⟨c, lm2⟩
+      specialize req1_true c
+      specialize req1_neg p c
+      specialize lm1 c
+      simp at lm1
+-/
+
+
+end IsSatRelAt
+
+
+
+abbrev IsSatRel {E AP: Type _} [Fintype AP] [EvalLike E AP] (rel: E → Formula AP → Prop) : Prop := IsSatRelAt AP E EvalLike.toIndicator rel
+
+
+structure SatRel (E AP: Type _) [Fintype AP] [EvalLike E AP] where
+  rel : E → Formula AP → Prop
+  valid: IsSatRel rel
+
+
+namespace SatRel
+
+open EvalLike
+
+variable {E AP: Type _} [Fintype AP] [EvalLike E AP] (sr: SatRel E AP) (μ: E)
+
+
+instance : FunLike (SatRel E AP) E (Formula AP → Prop) where
+  coe sr := sr.rel
+  coe_injective := by
+    rintro ⟨rel1⟩ ⟨rel2⟩
+    simp
+
+theorem app_eq_raw_app
+  : sr μ = sr.rel μ :=
+  rfl
+
+abbrev IsSat (p: Formula AP) : Prop := sr μ p
+
+section Notation
+
+syntax:25 term:26 " ⊨ₚ{" term "} " term:25 : term
+syntax:25 term:26 " ⊭ₚ{" term "} " term:25 : term
+
+macro_rules
+  | `( $μ ⊨ₚ{ $sr } $φ ) => ``(SatRel.IsSat $sr $μ $φ)
+  | `( $μ ⊭ₚ{ $sr } $φ ) => ``(¬($μ ⊨ₚ{ $sr } $φ))
+
+end Notation
+
+namespace IsSat
+
+@[scoped grind .]
+theorem true_intro
+  : μ ⊨ₚ{sr} (.true) := by
+  simp only [IsSat, app_eq_raw_app]
+  exact sr.valid.true μ
+
+@[scoped grind =]
+theorem atom_iff (a: AP)
+  : μ ⊨ₚ{sr} (.atom a) ↔ (toIndicator μ) a = .true := by
+  simp only [IsSat, app_eq_raw_app]
+  rw [sr.valid.atom]
+
+@[scoped grind =]
+theorem neg_iff (p: Formula AP)
+  : μ ⊨ₚ{sr} (¬ₚp) ↔ μ ⊭ₚ{sr} p := by
+  simp only [IsSat, app_eq_raw_app _ μ]
+  rw [sr.valid.neg]
+
+@[scoped grind =]
+theorem false_iff
+  : μ ⊨ₚ{sr} (.false) ↔ False := by
+  simp only [Formula.false]
+  grind only [= neg_iff, true_intro]
+
+@[scoped grind =]
+theorem and_iff (p1 p2: Formula AP)
+  : μ ⊨ₚ{sr} (p1 ∧ₚ p2) ↔ (μ ⊨ₚ{sr} p1) ∧ (μ ⊨ₚ{sr} p2) := by
+  simp only [IsSat, app_eq_raw_app _ μ]
+  rw [sr.valid.and]
+
+@[scoped grind =]
+theorem or_iff (p1 p2: Formula AP)
+  : μ ⊨ₚ{sr} (p1 ∨ₚ p2) ↔ (μ ⊨ₚ{sr} p1) ∨ (μ ⊨ₚ{sr} p2) := by
+  simp only [Formula.or]
+  grind
+
+theorem imp_iff_or (p1 p2: Formula AP)
+  : μ ⊨ₚ{sr} (p1 →ₚ p2) ↔ (μ ⊭ₚ{sr} p1) ∨ (μ ⊨ₚ{sr} p2) := by
+  simp only [Formula.imp]
+  grind
+
+@[scoped grind =]
+theorem imp_iff_imp (p1 p2: Formula AP)
+  : μ ⊨ₚ{sr} (p1 →ₚ p2) ↔ ((μ ⊨ₚ{sr} p1) → (μ ⊨ₚ{sr} p2)) := by
+  simp only [imp_iff_or]
+  grind only
+
+end IsSat
+
+
+
+
+
+/-- `p1` `p2` are semantically equivalent -/
+def SemEquiv (p1 p2: Formula AP) : Prop := ∀(μ: E), (μ ⊨ₚ{sr} p1) ↔ (μ ⊨ₚ{sr} p2)
+
+
+section Notation
+
+syntax:23 term:24 " ≡ₚ{" term "} " term:23 : term
+
+macro_rules
+  | `($p1 ≡ₚ{$sr} $p2) => ``(SemEquiv $sr $p1 $p2)
+
+end Notation
+
+@[scoped grind =]
+theorem semEquiv_iff (p1 p2: Formula AP) : sr.SemEquiv p1 p2 ↔ (∀(μ: E), (μ ⊨ₚ{sr} p1) ↔ (μ ⊨ₚ{sr} p2)) := by rfl
+
+namespace SemEquiv
+
+@[scoped grind ., refl]
+theorem refl (p: Formula AP) : (p ≡ₚ{sr} p) := by
+  unfold SemEquiv
+  intro _; rfl
+
+@[scoped grind →, symm]
+theorem symm (p1 p2: Formula AP) (h: (p1 ≡ₚ{sr} p2)) : p2 ≡ₚ{sr} p1 := by
+  revert h
+  unfold SemEquiv
+  intro h μ
+  symm
+  exact h μ
+
+@[scoped grind →]
+theorem trans (p1 p2 p3: Formula AP)
+  (h1: (p1 ≡ₚ{sr} p2)) (h2: (p2 ≡ₚ{sr} p3))
+  : p1 ≡ₚ{sr} p3 := by
+  revert h1 h2
+  unfold SemEquiv
+  intro h1 h2 μ
+  specialize h1 μ
+  specialize h2 μ
+  exact Iff.trans h1 h2
+
+theorem eqv : Equivalence (· ≡ₚ{sr} ·) where
+  refl := SemEquiv.refl sr
+  symm := SemEquiv.symm sr _ _
+  trans := SemEquiv.trans sr _ _ _
+
+instance : IsEquiv (Formula AP) (· ≡ₚ{sr} ·) := IsEquiv.of_equivalence (SemEquiv.eqv sr)
+
+
+
+@[reducible]
+def toSetoid : Setoid (Formula AP) where
+  r := sr.SemEquiv
+  iseqv := SemEquiv.eqv sr
+
+
+open scoped IsSat
+
+@[scoped grind .]
+theorem neg_neg (p: Formula AP)
+  : ¬ₚ¬ₚp ≡ₚ{sr} p := by
+  grind only [= semEquiv_iff, → symm, = IsSat.neg_iff]
+
+@[scoped grind .]
+theorem id_or (p: Formula AP)
+  : p ∨ₚ p ≡ₚ{sr} p := by
+  grind only [= semEquiv_iff, → symm, = IsSat.or_iff]
+
+@[scoped grind .]
+theorem id_and (p: Formula AP)
+  : p ∧ₚ p ≡ₚ{sr} p := by
+  grind only [= semEquiv_iff, → symm, = IsSat.and_iff]
+
+@[scoped grind .]
+theorem absorb_and (p1 p2: Formula AP)
+  : p1 ∧ₚ (p2 ∨ₚ p1) ≡ₚ{sr} p1 := by
+  grind only [= semEquiv_iff, → symm, = IsSat.and_iff, = IsSat.or_iff]
+
+@[scoped grind .]
+theorem absorb_or (p1 p2: Formula AP)
+  : p1 ∨ₚ (p2 ∧ₚ p1) ≡ₚ{sr} p1 := by
+  grind only [= semEquiv_iff, → symm, = IsSat.or_iff, = IsSat.and_iff]
+
+@[scoped grind .]
+theorem comm_or (p1 p2: Formula AP)
+  : p1 ∨ₚ p2 ≡ₚ{sr} p2 ∨ₚ p1 := by
+  grind only [= semEquiv_iff, → symm, = IsSat.or_iff]
+
+@[scoped grind .]
+theorem comm_and (p1 p2: Formula AP)
+  : p1 ∧ₚ p2 ≡ₚ{sr} p2 ∧ₚ p1 := by
+  grind only [= semEquiv_iff, → symm, = IsSat.and_iff]
+
+@[scoped grind .]
+theorem assoc_and (p1 p2 p3: Formula AP)
+  : p1 ∧ₚ (p2 ∧ₚ p3) ≡ₚ{sr} (p1 ∧ₚ p2) ∧ₚ p3 := by
+  grind only [= semEquiv_iff, → symm, = IsSat.and_iff]
+
+@[scoped grind .]
+theorem assoc_or (p1 p2 p3: Formula AP)
+  : p1 ∨ₚ (p2 ∨ₚ p3) ≡ₚ{sr} (p1 ∨ₚ p2) ∨ₚ p3 := by
+  grind only [= semEquiv_iff, → symm, = IsSat.or_iff]
+
+@[scoped grind .]
+theorem demorgan_and (p1 p2: Formula AP)
+  : ¬ₚ(p1 ∧ₚ p2) ≡ₚ{sr} (¬ₚp1 ∨ₚ ¬ₚp2) := by
+  grind only [= semEquiv_iff, → symm, = IsSat.neg_iff, = IsSat.or_iff, = IsSat.and_iff]
+
+@[scoped grind .]
+theorem demorgan_or (p1 p2: Formula AP)
+  : ¬ₚ(p1 ∨ₚ p2) ≡ₚ{sr} (¬ₚp1 ∧ₚ ¬ₚp2) := by
+  grind only [= semEquiv_iff, → symm, = IsSat.neg_iff, = IsSat.and_iff, = IsSat.or_iff]
+
+@[scoped grind .]
+theorem dist_or (p1 p2 p3: Formula AP)
+  : p1 ∨ₚ (p2 ∧ₚ p3) ≡ₚ{sr} (p1 ∨ₚ p2) ∧ₚ (p1 ∨ₚ p3) := by
+  grind
+
+@[scoped grind .]
+theorem dist_and (p1 p2 p3: Formula AP)
+  : p1 ∧ₚ (p2 ∨ₚ p3) ≡ₚ{sr} (p1 ∧ₚ p2) ∨ₚ (p1 ∧ₚ p3) := by
+  grind
+
+@[scoped grind .]
+theorem iterAnd_nil : ⋀ₚ ([]: List (Formula AP)) ≡ₚ{sr} (.true) := by
+  unfold Formula.iterAnd
+  rfl
+
+@[scoped grind .]
+theorem iterOr_nil : ⋁ₚ ([]: List (Formula AP)) ≡ₚ{sr} (.false) := by
+  unfold Formula.iterOr
+  rfl
+
+end SemEquiv
+
+def IsSatisfiable (p: Formula AP) : Prop := ∃(μ: E), μ ⊨ₚ{sr} p
+
+def IsValid (p: Formula AP) : Prop := ∀(μ: E), μ ⊨ₚ{sr} p
+
+abbrev IsUnsatisfiable (p: Formula AP) : Prop := ¬(sr.IsSatisfiable p)
+
+theorem unsatisfiable_iff_neg_valid (p: Formula AP)
+  : sr.IsUnsatisfiable p ↔ sr.IsValid (¬ₚp) := by
+  simp only [IsUnsatisfiable, IsSatisfiable, IsValid]
+  simp only [not_exists]
+  simp only [IsSat.neg_iff]
+
+
+protected def default : SatRel E AP where
+  rel := AreEvalToTrueAt E AP
+  valid := IsSatRelAt.of_eq_areEvalToTrue rfl
+
+
+instance toUnique : Unique (SatRel E AP) where
+  default := SatRel.default
+  uniq := by
+    rintro ⟨rel, valid⟩
+    dsimp [SatRel.default]
+    simp
+    dsimp [IsSatRel] at valid
+    exact valid.to_eq_areEvalToTrue
+
+
+def defaultAt (E AP: Type _) [Fintype AP] [EvalLike E AP] : SatRel E AP :=
+  (inferInstance: Unique (SatRel E AP)).toInhabited.default
+
+section Notation
+
+syntax:25 term:26 " ⊨ₚ " term:25 : term
+
+macro_rules
+  | `($μ ⊨ₚ $φ) => ``($μ ⊨ₚ{ defaultAt _ _ } $φ )
+
+
+syntax:25 term:26 " ⊨ₚ{ " term ", " term ", " term ", " term " }" term:25 : term
+
+macro_rules
+  | `($μ ⊨ₚ{ $EC , $AP , $ft , $el } $φ) => ``( @IsSat $EC $AP $ft $el (@defaultAt $EC $AP $ft $el) $μ $φ )
+
+
+syntax:25 term:26 " ⊨ₚ⟦ " term " ⟧ "  term:25 : term
+
+macro_rules
+  | `($μ ⊨ₚ⟦ $toInd ⟧ $φ) => ``( $μ ⊨ₚ{ _, _, _, EvalLike.ofKerLift $toInd } $φ )
+
+end Notation
+
+
+
+
+end SatRel
+
+/-
+namespace Formula
+
+class HasEvalLike (AP: Type*) [Fintype AP] where
+  Carrier: Type*
+  [evalLike: EvalLike Carrier AP]
+
+attribute [reducible] HasEvalLike.Carrier
+attribute [reducible, instance] HasEvalLike.evalLike
+
+namespace HasEvalLike
+
+def toSatRel (AP: Type*) [Fintype AP] [HasEvalLike AP] : SatRel (Carrier AP) AP :=
+  (inferInstance: Unique (SatRel (Carrier AP) AP)).toInhabited.default
+
+
+
+
+end HasEvalLike
+
+end Formula
+-/
+
+
+
+
+
+/-
+class HasSatRelAt {AP: Type _} [Fintype AP] (μ: Eval AP) (p: Formula AP) where
+  satRel: SatRel AP
+
+
+section Notation
+
+syntax:25 term:26 " ⊨ₚ " term:25 : term
+
+macro_rules
+  | `($μ ⊨ₚ $φ) => ``($μ ⊨ₚ{ HasSatRelAt.satRel $μ $φ } $φ )
+
+end Notation
+
+
+namespace HasSatRelAt
+
+variable {E AP: Type _} [Fintype AP] [EvalLike E AP]
+-/
+
+
+/-
+instance ofEvalLike (e: E) (p: Formula AP) : HasSatRelAt (e: Eval AP) p where
+  satRel := {
+    rel :=
+    valid := _
+  }
+-/
+
+
+
+
+/-
+class SatRelLike (SR: Type _) (E: Type _) (AP: outParam <| Type _) [Fintype AP] [EvalLike E AP] where
+  toRel : SR → E → Formula AP → Prop
+  valid (sr: SR) : IsSatRel AP (fun ev => toRel sr (EvalLike.coeInv ev))
+-/
+/-
+  true (sr: SR) : ∀μ, toRel sr μ (.true)
+  atom (sr: SR) (a: AP) : ∀μ, toRel sr μ (.atom a) ↔ ((μ: Eval AP) a = .true)
+  neg (sr: SR) (x: Formula AP) : ∀μ, toRel sr μ (¬ₚx) ↔ (¬toRel sr μ x)
+  and (sr: SR) (x y: Formula AP) : ∀μ, toRel sr μ (x ∧ₚ y) ↔ (toRel sr μ x ∧ toRel sr μ y)
+-/
+
+/-
+namespace SatRelLike
+
+variable {SR E AP: Type _} [Fintype AP] [EvalLike E AP] [SatRelLike SR E AP]
+
+
+def toSatRel (sr: SR) : SatRel AP where
+  rel ev := toRel sr (EvalLike.coeInv ev : E)
+  valid := SatRelLike.valid sr
+
+#print toSatRel
+
+
+end SatRelLike
+-/
+
+end Nemonuri.PropositionalLogics
+
+end
