Nemonuri/PropositionalLogics/Tactic.lean
@@ -1,0 +1,22 @@
+module
+
+public meta import Nemonuri.PropositionalLogics.Attributes
+public import Nemonuri.PropositionalLogics.Basic
+
+@[expose] public section
+
+namespace Nemonuri.PropositionalLogics
+
+namespace SatRel.IsSat
+
+attribute [pl_simp] true_intro atom_iff neg_iff false_iff and_iff or_iff imp_iff_imp
+
+end SatRel.IsSat
+
+attribute [pl_simp] EvalLike.toIndicator_def
+
+attribute [pl_simp low] Indicator.mk_fn_eq Indicator.mk_eq
+
+end Nemonuri.PropositionalLogics
+
+end
